Examples/LockResource/LockPrograms.v
@@ -1,0 +1,140 @@
+From mathcomp.ssreflect
+Require Import ssreflect ssrbool ssrnat eqtype ssrfun seq.
+From mathcomp
+Require Import path.
+Require Import Eqdep.
+Require Import pred prelude idynamic ordtype finmap pcm unionmap heap coding domain.
+Require Import Freshness State EqTypeX Protocols Worlds NetworkSem Rely.
+Require Import Actions.
+Require Import SeqLib.
+Require Import StatePredicates.
+Require Import Actions Injection Process Always HoareTriples InferenceRules.
+
+Require Import LockProtocol LockSmallWorld.
+
+Module L := LockProtocol.
+Module LSW := LockSmallWorld.
+
+Set Implicit Arguments.
+Unset Strict Implicit.
+Import Prenex Implicits.
+
+Section LockPrograms.
+
+Variable (l : Label).
+Variable (server : nid) (clients : seq nid).
+Hypothesis server_not_client : server \notin clients.
+
+Variable this : nid.
+Hypothesis this_in_clients : this \in clients.
+
+Notation this_not_server := (LSW.this_not_server server_not_client this_in_clients).
+
+Notation protocol := (LockProtocol server_not_client l).
+Notation W := (@LSW.W l server clients server_not_client).
+
+Program Definition send_acquire_act :=
+  act (@send_action_wrapper W protocol this l _
+        (L.client_send_acquire_trans server_not_client)
+        _
+        [::]
+        server).
+Next Obligation. by rewrite /getProtocol/W/= um_findPt. Qed.
+Next Obligation. by rewrite !InE; right; left. Qed.
+
+Definition acquire_perms (p : seq nid -> Prop) d :=
+  exists s : L.server_state,
+    getLocal server d = L.st :-> s /\
+    p (L.outstanding s).
+
+Definition no_pending_acquires :=
+  acquire_perms (fun out => this \notin out).
+
+Definition lock_init_state d :=
+  [/\ L.not_held this d,
+     no_pending_acquires d,
+     no_msg_from_to this server (dsoup d) &
+     no_msg_from_to server this (dsoup d)].
+
+Definition acquire_sent d :=
+  [/\ L.not_held this d,
+     msg_spec this server L.acquire_tag [::] (dsoup d),
+     no_pending_acquires d &
+     no_msg_from_to server this (dsoup d)].
+
+Definition outstanding_acquire :=
+  acquire_perms (fun out => count_mem this out = 1).
+
+Definition acquire_pending d :=
+  [/\ L.not_held this d,
+     no_msg_from_to this server (dsoup d),
+     outstanding_acquire d &
+     no_msg_from_to server this (dsoup d)].
+
+Definition grant_sent d :=
+  [/\ L.not_held this d,
+     no_msg_from_to this server (dsoup d),
+     no_pending_acquires d &
+     exists e, msg_spec server this L.grant_tag [:: e] (dsoup d)].
+
+Definition lock_request_in_flight d :=
+  [\/ acquire_sent d,
+     acquire_pending d |
+     grant_sent d].
+
+Lemma lock_init_state_rely s1 s2 :
+  network_rely W this s1 s2 ->
+  lock_init_state (getStatelet s1 l) ->
+  lock_init_state (getStatelet s2 l).
+Admitted.
+
+Lemma lock_request_in_flight_rely s1 s2 :
+  network_rely W this s1 s2 ->
+  lock_request_in_flight (getStatelet s1 l) ->
+  lock_request_in_flight (getStatelet s2 l).
+Admitted.
+
+Program Definition send_acquire :
+  DHT [this, W]
+    (fun i => lock_init_state (getStatelet i l),
+     fun r m => lock_request_in_flight (getStatelet m l))
+  := Do send_acquire_act.
+Next Obligation.
+move=>s0/= Init0.
+apply: act_rule=>s1 Rely01; split=>/=.
+- rewrite /Actions.send_act_safe/=.
+  move/rely_coh: (Rely01)=> [_ C1].
+  move: (coh_coh l C1); rewrite LSW.W_l/==>Cs1.
+  split=>//; [split=>// | | ].
+  + rewrite /L.client_send_acquire_prec.
+    have HC: L.HClient server clients this server by [].
+    exists HC, Cs1.
+    rewrite (L.getSt_client_K(m:=L.NotHeld) _ Cs1 _ this_in_clients)//.
+    by move: Init0=>[] H; rewrite (not_held_rely Rely01)//.
+  + apply/andP; split=>//=; first by rewrite -(cohD C1) LSW.W_dom !inE eqxx.
+    by rewrite inE this_in_clients orbC.
+  by move=>z lc hk; rewrite find_um_filt eqxx find0E.
+move=>m s2 s3 [Safe] Step Rely23 _.
+apply /(lock_request_in_flight_rely Rely23).
+constructor 1.
+move: (lock_init_state_rely Rely01 Init0).
+rewrite /lock_init_state/acquire_sent=>-[NH1 NP1 NM1 NM'1].
+case: Step=>_/=[h'][h'def]s2def.
+have C1 := (rely_coh Rely01).2.
+have Cs1 := (coh_coh l C1).
+rewrite s2def /getStatelet findU eqxx/= (cohS C1) /= getsE;
+  last by rewrite -(cohD C1) LSW.W_dom !inE/= eqxx.
+split.
+- rewrite /L.not_held/getLocal/= findU eqxx/= (cohVl Cs1).
+  by move: h'def; rewrite /L.client_step/L.client_send_step=>-[].
+- apply /msg_specE=>//.
+  by apply /(cohVs Cs1).
+- move: NP1.
+  rewrite /no_pending_acquires/acquire_perms.
+  by rewrite /getLocal/= findU (negbTE this_not_server).
+apply /no_msg_from_toE'=>//.
+by apply /(cohVs Cs1).
+by rewrite eq_sym; apply/negbTE/this_not_server.
+Qed.
+
+End LockPrograms.
