Examples/LockResource/LockSmallWorld.v
@@ -1,0 +1,84 @@
+From mathcomp.ssreflect
+Require Import ssreflect ssrbool ssrnat eqtype ssrfun seq.
+From mathcomp
+Require Import path.
+Require Import Eqdep.
+Require Import pred prelude idynamic ordtype finmap pcm unionmap heap coding domain.
+Require Import Freshness State EqTypeX Protocols Worlds NetworkSem Rely.
+Require Import Actions.
+Require Import SeqLib.
+Require Import StatePredicates.
+Require Import Actions Injection Process Always HoareTriples InferenceRules.
+
+Require Import LockProtocol.
+
+Module L := LockProtocol.
+
+Set Implicit Arguments.
+Unset Strict Implicit.
+Import Prenex Implicits.
+
+Module LockSmallWorld.
+Section LockSmallWorld.
+
+Variable (l : Label).
+Variable (server : nid) (clients : seq nid).
+Hypothesis server_not_client : server \notin clients.
+
+Variable this : nid.
+Hypothesis this_in_clients : this \in clients.
+
+Lemma this_not_server :
+  server != this.
+Proof.
+  case X: (server == this)=>//.
+  move/eqP in X.
+  move: (this_in_clients) (server_not_client).
+  by rewrite X=>->.
+Qed.
+
+Notation protocol := (LockProtocol server_not_client l).
+
+Definition W : world := (l \\-> protocol, Unit).
+
+Lemma W_valid : valid W.
+Proof. by apply /andP; split=>//=; rewrite um_validPt. Qed.
+
+Lemma W_complete : hook_complete W.
+Proof. by move=>z lc ls t/=; rewrite dom0. Qed.
+
+Lemma W_dom : dom W.1 =i [:: l].
+Proof. by move=>z/=; rewrite um_domPt !inE eq_sym. Qed.
+
+Lemma W_l : getProtocol W l = protocol.
+Proof. by rewrite /getProtocol/W/= um_findPt. Qed.
+
+Notation assert_local this x d := (getLocal this d = L.st :-> x).
+
+Lemma assert_local_rely A (x : A) s1 s2 :
+  network_rely W this s1 s2 ->
+  assert_local this x (getStatelet s1 l) ->
+  assert_local this x (getStatelet s2 l).
+Proof. by move=>Rely12; rewrite (rely_loc' _ Rely12). Qed.
+
+Lemma held_rely e s1 s2 :
+  network_rely W this s1 s2 ->
+  L.held this e (getStatelet s1 l) ->
+  L.held this e (getStatelet s2 l).
+Proof. exact: assert_local_rely. Qed.
+
+Lemma not_held_rely s1 s2 :
+  network_rely W this s1 s2 ->
+  L.not_held this (getStatelet s1 l) ->
+  L.not_held this (getStatelet s2 l).
+Proof. exact: assert_local_rely. Qed.
+
+End LockSmallWorld.
+Module Exports.
+Definition held_rely := held_rely.
+Definition not_held_rely := not_held_rely.
+End Exports.
+End LockSmallWorld.
+
+Export LockSmallWorld.Exports.
+
